src/Examples/Interprocedural/Example_Proc_Call.thy
@@ -29,7 +29,7 @@ definition sqr_body :: "IMP2_Proc.com" where
   "sqr_body = imp \<lbrakk> Gx := Gx * Gx \<rbrakk>"
 
 definition proc_pi :: proc_table where
-  "proc_pi = (\<lambda>_. None)(''inc'' := Some (proc_decl_of [] inc_body None), ''sqr'' := Some (proc_decl_of [] sqr_body None))"
+  "proc_pi = (\<lambda>_. None)(''inc'' := Some (proc_decl_of [] inc_body), ''sqr'' := Some (proc_decl_of [] sqr_body))"
 
 definition main_prog :: "IMP2_Proc.com" where
   "main_prog = imp \<lbrakk>
@@ -54,7 +54,7 @@ proof -
   have run: "pcompletes proc_pi (IMP2_Proc.Call None ''inc'' []) s
                 (IMP2_Globals.combine_states s ((enter_state s)(''Gx'' := s ''Gx'' + 1)))"
   proof (rule pcompletes_Call_parameterless[where c = inc_body])
-    show "proc_pi ''inc'' = Some (proc_decl_of [] inc_body None)"
+    show "proc_pi ''inc'' = Some (proc_decl_of [] inc_body)"
       by (simp add: proc_pi_def)
     show "pcompletes proc_pi inc_body (enter_state s)
              ((enter_state s)(''Gx'' := s ''Gx'' + 1))"
@@ -79,7 +79,7 @@ proof -
   have run: "pcompletes proc_pi (IMP2_Proc.Call None ''sqr'' []) s
                 (IMP2_Globals.combine_states s ((enter_state s)(''Gx'' := s ''Gx'' * s ''Gx'')))"
   proof (rule pcompletes_Call_parameterless[where c = sqr_body])
-    show "proc_pi ''sqr'' = Some (proc_decl_of [] sqr_body None)"
+    show "proc_pi ''sqr'' = Some (proc_decl_of [] sqr_body)"
       by (simp add: proc_pi_def)
     show "pcompletes proc_pi sqr_body (enter_state s)
              ((enter_state s)(''Gx'' := s ''Gx'' * s ''Gx''))"
